common/Memstructure.v
@@ -9,9 +9,123 @@ Require Import Values.
 Require Export Memdata.
 Require Export Memtype.
 Require Export Memory.
+
 (* To avoid useless definitions of inductors in extracted code. *)
 Local Unset Elimination Schemes.
 Local Unset Case Analysis Schemes.
+
+Module Pos_Block <: BLOCK.
+
+Definition block := positive.
+Definition eq_block := peq.
+
+End Pos_Block.
+
+Module MemPos.
+Include Mem(Pos_Block).
+
+Fixpoint find_max_pos (l: list positive) : positive :=
+  match l with
+  |nil => 1
+  |hd::tl => let m' := find_max_pos tl in
+             match plt hd m' with
+             |left _ => m'
+             |right _ => hd
+             end
+  end.
+
+Theorem Lessthan: forall p l, In p l -> Ple p (find_max_pos l).
+Proof.
+  intros.
+  induction l.
+  destruct H.
+  destruct H;simpl.
+  - destruct (plt a (find_max_pos l)); subst a.
+    + apply Plt_Ple. assumption.
+    + apply Ple_refl.
+  - destruct (plt a (find_max_pos l)); apply IHl in H.
+    + auto.
+    + eapply Ple_trans. eauto.  apply Pos.le_nlt. apply n.
+Qed.
+
+Definition fresh_block (l: list ident) := Pos.succ (find_max_pos l).
+
+Theorem freshness : forall s, ~In (fresh_block s) s.
+Proof.
+  intros. unfold fresh_block.
+  intro.
+  apply Lessthan in H.
+  assert (Plt (find_max_pos s) (Pos.succ (find_max_pos s))). apply Plt_succ.
+  assert (Plt (find_max_pos s) (find_max_pos s)). eapply Plt_Ple_trans. eauto. auto.
+  apply Plt_strict in H1.
+  auto.
+Qed.
+
+Lemma fresh_ne : forall (b:block)(s:sup), In b s -> b <> fresh_block s.
+Proof.
+  intros. destruct (eq_block b (fresh_block s)).
+  - rewrite e in H. apply freshness in H. destruct H.
+  - auto.
+Qed.
+
+End MemPos.
+
+Opaque MemPos.alloc MemPos.free MemPos.store MemPos.load MemPos.storebytes MemPos.loadbytes.
+
+ Hint Resolve
+  MemPos.valid_not_valid_diff
+  MemPos.perm_implies
+  MemPos.perm_cur
+  MemPos.perm_max
+  MemPos.perm_valid_block
+  MemPos.range_perm_implies
+  MemPos.range_perm_cur
+  MemPos.range_perm_max
+  MemPos.valid_access_implies
+  MemPos.valid_access_valid_block
+  MemPos.valid_access_perm
+  MemPos.valid_access_load
+  MemPos.load_valid_access
+  MemPos.loadbytes_range_perm
+  MemPos.valid_access_store
+  MemPos.perm_store_1
+  MemPos.perm_store_2
+  MemPos.store_valid_block_1
+  MemPos.store_valid_block_2
+  MemPos.store_valid_access_1
+  MemPos.store_valid_access_2
+  MemPos.store_valid_access_3
+  MemPos.storebytes_range_perm
+  MemPos.perm_storebytes_1
+  MemPos.perm_storebytes_2
+  MemPos.storebytes_valid_access_1
+  MemPos.storebytes_valid_access_2
+  MemPos.storebytes_valid_block_1
+  MemPos.storebytes_valid_block_2
+  MemPos.valid_block_alloc
+  MemPos.fresh_block_alloc
+  MemPos.valid_new_block
+  MemPos.perm_alloc_1
+  MemPos.perm_alloc_2
+  MemPos.perm_alloc_3
+  MemPos.perm_alloc_4
+  MemPos.perm_alloc_inv
+  MemPos.valid_access_alloc_other
+  MemPos.valid_access_alloc_same
+  MemPos.valid_access_alloc_inv
+  MemPos.range_perm_free
+  MemPos.free_range_perm
+  MemPos.valid_block_free_1
+  MemPos.valid_block_free_2
+  MemPos.perm_free_1
+  MemPos.perm_free_2
+  MemPos.perm_free_3
+  MemPos.valid_access_free_1
+  MemPos.valid_access_free_2
+  MemPos.valid_access_free_inv_1
+  MemPos.valid_access_free_inv_2
+  MemPos.unchanged_on_refl
+: mem.
 
 (* Module Type SUP(Block:BLOCK).
 Include Block.
@@ -55,7 +169,7 @@ Proof.
 Qed.
 
 End SUP.*)
-
+(* WIP: 3part mem
 Module Memstructure1.
 
 Module Block <: BLOCK.
@@ -95,7 +209,7 @@ Definition structure_In (b:block)(s:structure) :=
   end.
 
 
-Definition match_mem_structure (m:Mem.mem) (s:structure) :=
+Definition match_mem_structure (m:MemPos.mem) (s:structure) :=
    forall b, Mem.valid_block m b <-> structure_In b s.
 
 Fixpoint find_max_pos (l: list positive) : positive :=
@@ -136,5 +250,5 @@ Proof.
 Qed.
 
 End Memstructure1.
-
+*)
 
