backend/CminorSel.v
@@ -432,8 +432,9 @@ Inductive step: state -> trace -> state -> Prop :=
       step (State f (Sgoto lbl) k sp e m)
         E0 (State f s' k' sp e m)
 
-  | step_internal_function: forall f vargs k m m' sp e,
-      Mem.alloc m 0 f.(fn_stackspace) = (m', sp) ->
+  | step_internal_function: forall f vargs k m m' sp e
+      (SP: sp = fresh_block (support m)),
+      Mem.alloc m 0 f.(fn_stackspace) sp = Some m' ->
       set_locals f.(fn_vars) (set_params vargs f.(fn_params)) = e ->
       step (Callstate (Internal f) vargs k m)
         E0 (State f f.(fn_body) k (Vptr sp Ptrofs.zero) e m')
