backend/RTL.v
@@ -268,8 +268,9 @@ Inductive step: state -> trace -> state -> Prop :=
       step (State s f (Vptr stk Ptrofs.zero) pc rs m)
         E0 (Returnstate s (regmap_optget or Vundef rs) m')
   | exec_function_internal:
-      forall s f args m m' stk,
-      Mem.alloc m 0 f.(fn_stacksize) = (m', stk) ->
+      forall s f args m m' stk
+      (STK: stk = fresh_block(support m)),
+      Mem.alloc m 0 f.(fn_stacksize) stk = Some m' ->
       step (Callstate s (Internal f) args m)
         E0 (State s
                   f
