common/Builtins.v
@@ -20,8 +20,6 @@ Require Import String Coqlib.
 Require Import AST Integers Floats Values.
 Require Export Builtins0 Builtins1.
 
-Module Builtins(Block:BLOCK).
-Include Builtins1(Block).
 Inductive builtin_function : Type :=
   | BI_standard (b: standard_builtin)
   | BI_platform (b: platform_builtin).
@@ -57,6 +55,6 @@ Proof.
   inv H. simpl. eapply lookup_builtin_sig; eauto.
   discriminate.
 Qed.
-End Builtins.
+
 
 
