common/Switch.v
@@ -22,7 +22,8 @@ Require Import Coqlib.
 Require Import Maps.
 Require Import Integers.
 Require Import Values.
-
+Require Import Memstructure.
+Import MemPos.
 (** A multi-way branch is composed of a list of (key, action) pairs,
   plus a default action.  *)
 
